
\documentclass[12pt,a4paper]{article}
\usepackage{amsmath}

\begin{document}
In the original paper the MDCEV model is defined as
\begin{equation}
  P\left(t_2^*, t_3^*, \ldots, t_M^*, 0,0, \ldots, 0\right)=
  \left[\prod_{i=1}^M c_i\right]
  \left[\sum_{i=1}^M \frac{1}{c_i}\right]
  \left[\frac{\prod_{i=1}^M e^{V_i}}{\left(\sum_{j=1}^K e^{V_j}\right)^M}\right](M-1) !,
\end{equation}
where
\begin{equation}
  V_j=\beta^{\prime} x_j+\ln \alpha_j+\left(\alpha_j-1\right) \ln \left(t_j^*+\gamma_j\right)
\end{equation}
and
\begin{equation}
  c_i=\left(\frac{1-\alpha_i}{t_i^*+\gamma_i}\right)
\end{equation}

In the 2007 paper, it is defined as follows:
\begin{equation}
  \begin{aligned}
P\left(e_1^*, e_2^*, e_3^*, \ldots, e_M^*, 0,0, \ldots, 0\right) = &\\
\frac{1}{\sigma^{M-1}}
\left[\prod_{i=1}^M c_i\right]
\left[\sum_{i=1}^M \frac{1}{c_i}\right]
\left[\frac{\prod_{i=1}^M e^{V_i / \sigma}}{\left(\sum_{k=1}^K e^{V_k / \sigma}\right)^M}\right](M-1) !,
  \end{aligned}
\end{equation}

where
\begin{equation}
  V_k=\beta^{\prime} z_k+\left(\alpha_k-1\right) \ln \left(\frac{e_k^*}{p_k}+1\right)-\ln p_k
\end{equation}
and
  \begin{equation}
    c_i=\left(\frac{1-\alpha_i}{e_i^*+\gamma_i p_i}\right).
  \end{equation}
\end{document}
